rocq/theories/TypeSystem/TypeChecker.v
@@ -3662,6 +3662,22 @@ Fixpoint duplicate_param_name_aux (seen : list string) (ps : list param) : optio
 Definition duplicate_param_name (ps : list param) : option ident :=
   duplicate_param_name_aux [] ps.
 
+Definition fn_binding_params (f : fn_def) : list param :=
+  fn_captures f ++ fn_params f.
+
+Definition check_fn_binding_params (Δ : region_ctx) (f : fn_def)
+    : option infer_error :=
+  if negb (wf_params_b Δ (fn_captures f))
+  then Some ErrLifetimeLeak
+  else
+  if negb (wf_params_b Δ (fn_params f))
+  then Some ErrLifetimeLeak
+  else
+  match duplicate_param_name (fn_binding_params f) with
+  | Some x => Some (ErrDuplicateParam x)
+  | None => None
+  end.
+
 Lemma string_in_false_not_in : forall x xs,
   string_in x xs = false ->
   ~ In x xs.
@@ -3747,6 +3763,14 @@ Proof.
   - simpl. rewrite IH. reflexivity.
 Qed.
 
+Lemma param_names_app : forall ps1 ps2,
+  param_names (ps1 ++ ps2) = param_names ps1 ++ param_names ps2.
+Proof.
+  induction ps1 as [| p ps1 IH]; intros ps2.
+  - reflexivity.
+  - simpl. rewrite IH. reflexivity.
+Qed.
+
 Lemma duplicate_param_name_aux_none_no_seen : forall seen ps x,
   duplicate_param_name_aux seen ps = None ->
   In x (param_names ps) ->
@@ -3793,6 +3817,19 @@ Proof.
   exact Hnone.
 Qed.
 
+Lemma duplicate_param_name_none_nodup_params_ctx_suffix : forall caps ps,
+  duplicate_param_name (caps ++ ps) = None ->
+  NoDup (ctx_names (params_ctx ps)).
+Proof.
+  intros caps ps Hnone.
+  rewrite ctx_names_params_ctx_param_names.
+  pose proof (duplicate_param_name_none_nodup_params_ctx (caps ++ ps) Hnone)
+    as Hnodup_all.
+  rewrite ctx_names_params_ctx_param_names in Hnodup_all.
+  rewrite param_names_app in Hnodup_all.
+  eapply NoDup_app_right. exact Hnodup_all.
+Qed.
+
 
 (* Check a single function definition:
    - infer the body type
@@ -3812,11 +3849,8 @@ Definition infer (fenv : list fn_def) (f : fn_def)
   if negb (wf_type_b Δ (fn_ret f))
   then infer_err ErrLifetimeLeak
   else
-  if negb (wf_params_b Δ (fn_params f))
-  then infer_err ErrLifetimeLeak
-  else
-  match duplicate_param_name (fn_params f) with
-  | Some x => infer_err (ErrDuplicateParam x)
+  match check_fn_binding_params Δ f with
+  | Some err => infer_err err
   | None =>
   match infer_body fenv Ω n (params_ctx (fn_params f)) (fn_body f) with
   | infer_err err => infer_err err
@@ -3851,11 +3885,8 @@ Definition infer_env (env : global_env) (f : fn_def)
   if negb (wf_type_b Δ (fn_ret f))
   then infer_err ErrLifetimeLeak
   else
-  if negb (wf_params_b Δ (fn_params f))
-  then infer_err ErrLifetimeLeak
-  else
-  match duplicate_param_name (fn_params f) with
-  | Some x => infer_err (ErrDuplicateParam x)
+  match check_fn_binding_params Δ f with
+  | Some err => infer_err err
   | None =>
   match infer_core_env env Ω n (params_ctx (fn_params f)) (fn_body f) with
   | infer_err err => infer_err err
@@ -3886,11 +3917,8 @@ Definition infer_env_elab (env : global_env) (f : fn_def)
   if negb (wf_type_b Δ (fn_ret f))
   then infer_err ErrLifetimeLeak
   else
-  if negb (wf_params_b Δ (fn_params f))
-  then infer_err ErrLifetimeLeak
-  else
-  match duplicate_param_name (fn_params f) with
-  | Some x => infer_err (ErrDuplicateParam x)
+  match check_fn_binding_params Δ f with
+  | Some err => infer_err err
   | None =>
   match infer_core_env_elab env Ω n (params_ctx (fn_params f)) (fn_body f) with
   | infer_err err => infer_err err
@@ -3917,11 +3945,8 @@ Definition infer_env_roots (env : global_env) (f : fn_def) (R0 : root_env)
   if negb (wf_type_b Δ (fn_ret f))
   then infer_err ErrLifetimeLeak
   else
-  if negb (wf_params_b Δ (fn_params f))
-  then infer_err ErrLifetimeLeak
-  else
-  match duplicate_param_name (fn_params f) with
-  | Some x => infer_err (ErrDuplicateParam x)
+  match check_fn_binding_params Δ f with
+  | Some err => infer_err err
   | None =>
   match infer_core_env_roots env Ω n R0 (params_ctx (fn_params f)) (fn_body f) with
   | infer_err err => infer_err err
@@ -3949,11 +3974,8 @@ Definition infer_env_roots_shadow_safe
   if negb (wf_type_b Δ (fn_ret f))
   then infer_err ErrLifetimeLeak
   else
-  if negb (wf_params_b Δ (fn_params f))
-  then infer_err ErrLifetimeLeak
-  else
-  match duplicate_param_name (fn_params f) with
-  | Some x => infer_err (ErrDuplicateParam x)
+  match check_fn_binding_params Δ f with
+  | Some err => infer_err err
   | None =>
   match infer_core_env_roots_shadow_safe
           env Ω n R0 (params_ctx (fn_params f)) (fn_body f) with
@@ -3980,11 +4002,15 @@ Proof.
     try discriminate.
   destruct (negb (wf_type_b (mk_region_ctx (fn_lifetimes f)) (fn_ret f)));
     try discriminate.
+  unfold check_fn_binding_params in Hinfer.
+  destruct (negb (wf_params_b (mk_region_ctx (fn_lifetimes f)) (fn_captures f)));
+    try discriminate.
   destruct (negb (wf_params_b (mk_region_ctx (fn_lifetimes f)) (fn_params f)));
     try discriminate.
-  destruct (duplicate_param_name (fn_params f)) as [dup |] eqn:Hdup;
+  destruct (duplicate_param_name (fn_binding_params f)) as [dup |] eqn:Hdup;
     try discriminate.
-  apply duplicate_param_name_none_nodup_params_ctx. exact Hdup.
+  unfold fn_binding_params in Hdup.
+  eapply duplicate_param_name_none_nodup_params_ctx_suffix. exact Hdup.
 Qed.
 
 Lemma infer_env_roots_params_nodup : forall env f R0 T Γ' R' roots,
@@ -3997,11 +4023,15 @@ Proof.
     try discriminate.
   destruct (negb (wf_type_b (mk_region_ctx (fn_lifetimes f)) (fn_ret f)));
     try discriminate.
+  unfold check_fn_binding_params in Hinfer.
+  destruct (negb (wf_params_b (mk_region_ctx (fn_lifetimes f)) (fn_captures f)));
+    try discriminate.
   destruct (negb (wf_params_b (mk_region_ctx (fn_lifetimes f)) (fn_params f)));
     try discriminate.
-  destruct (duplicate_param_name (fn_params f)) as [dup |] eqn:Hdup;
+  destruct (duplicate_param_name (fn_binding_params f)) as [dup |] eqn:Hdup;
     try discriminate.
-  apply duplicate_param_name_none_nodup_params_ctx. exact Hdup.
+  unfold fn_binding_params in Hdup.
+  eapply duplicate_param_name_none_nodup_params_ctx_suffix. exact Hdup.
 Qed.
 
 Definition ex_struct_pair : struct_def :=
@@ -5104,11 +5134,8 @@ Definition infer_direct (fenv : list fn_def) (f : fn_def)
   if negb (wf_type_b Δ (fn_ret f))
   then infer_err ErrLifetimeLeak
   else
-  if negb (wf_params_b Δ (fn_params f))
-  then infer_err ErrLifetimeLeak
-  else
-  match duplicate_param_name (fn_params f) with
-  | Some x => infer_err (ErrDuplicateParam x)
+  match check_fn_binding_params Δ f with
+  | Some err => infer_err err
   | None =>
   match infer_core fenv Ω n (params_ctx (fn_params f)) (fn_body f) with
   | infer_err err => infer_err err
